Update
Signed-off-by: FedericoBruzzone <federico.bruzzone.i@gmail.com>

last_lesson/plf/terse/do.v
@@ -6,7 +6,6 @@ From Coq Require Import Arith.PeanoNat. Import Nat.
 From Coq Require Import Lia.
 From PLF Require Import Imp.
 
-
 (** Consider a version of Imp, where the assignment and skip command
 are _replaced_ with a new command [Do f], where [f : state -> state]
 is an arbitrary state transformation.
@@ -37,23 +36,42 @@ of assigment via [Do].
 [{{True}} X := 1 {{X = 1}}]
 *)
 
-Print state.
+Print com.
 
 Inductive com2 : Type :=
-  | CDo (f : (state -> state))
-  (* | CSkip *)
-  (* | CAsgn (x : string) (a : aexp) *)
-  | CSeq (c1 c2 : com2)
-  | CIf (b : bexp) (c1 c2 : com2)
-  | CWhile (b : bexp) (c : com2).
+    (* CSkip : com *)
+  (* | CAsgn : string -> aexp -> com *)
+  | CDo : (state -> state) -> com2
+  | CSeq : com2 -> com2 -> com2
+  | CIf : bexp -> com2 -> com2 -> com2
+  | CWhile : bexp -> com2 -> com2.
 
 Definition skip2 := CDo (fun st => st).
-Definition assgn2 (s: string) (a: aexp) := CDo (fun st => s !-> (aeval st a) ; st).
+Definition asgn2(s : string) (a : aexp) := CDo (fun st => (t_update st s (aeval st a))).
+
+Notation "'skip2'"  :=
+         skip2 (in custom com at level 0) : com_scope.
+Notation "s ::= a"  :=
+         (asgn2 s a)
+            (in custom com at level 0, s constr at level 0,
+             a at level 85, no associativity) : com_scope.
+Notation "x ; y" :=
+         (CSeq x y)
+           (in custom com at level 90,
+            right associativity) : com_scope.
+Notation "'if' x 'then' y 'else' z 'end'" :=
+         (CIf x y z)
+           (in custom com at level 89, x at level 99,
+            y at level 99, z at level 99) : com_scope.
+Notation "'while' x 'do' y 'end'" :=
+         (CWhile x y)
+           (in custom com at level 89, x at level 99,
+            y at level 99) : com_scope.
 
 Reserved Notation
-  "st '==[' c ']=>' st'"
-  (at level 40, c custom com at level 99,
-  st constr, st' constr at next level).
+    "st '==[' c ']=>' st'"
+     (at level 40, c custom com at level 99,
+     st constr, st' constr at next level).
 
 Inductive ceval2 : com2 -> state -> state -> Prop :=
   (* | E_Skip : forall st, *)
@@ -61,74 +79,193 @@ Inductive ceval2 : com2 -> state -> state -> Prop :=
   (* | E_Asgn  : forall st a n x, *)
   (*     aeval st a = n -> *)
   (*     st =[ x := a ]=> (x !-> n ; st) *)
-  | E_CDo : forall f st st',
-      st' = f st ->
-      st ==[ CDo f ]=> st'
+  | E_Do : forall f st,
+      st ==[ CDo f ]=> f st
   | E_Seq : forall c1 c2 st st' st'',
       st  ==[ c1 ]=> st'  ->
       st' ==[ c2 ]=> st'' ->
-      st  ==[ CSeq c1 c2 ]=> st''
+      st  ==[ c1 ; c2 ]=> st''
   | E_IfTrue : forall st st' b c1 c2,
       beval st b = true ->
       st ==[ c1 ]=> st' ->
-      st ==[ CIf b c1 c2 ]=> st'
+      st ==[ if b then c1 else c2 end]=> st'
   | E_IfFalse : forall st st' b c1 c2,
       beval st b = false ->
       st ==[ c2 ]=> st' ->
-      st ==[ CIf b c1 c2 ]=> st'
+      st ==[ if b then c1 else c2 end]=> st'
   | E_WhileFalse : forall b st c,
       beval st b = false ->
-      st ==[ CWhile b c ]=> st
+      st ==[ while b do c end ]=> st
   | E_WhileTrue : forall st st' st'' b c,
       beval st b = true ->
       st  ==[ c ]=> st' ->
-      st' ==[ CWhile b c ]=> st'' ->
-      st  ==[ CWhile b c ]=> st''
-    where "st ==[ c ]=> st'" := (ceval2 c st st').
+      st' ==[ while b do c end ]=> st'' ->
+      st  ==[ while b do c end ]=> st''
 
-Theorem der_skip: forall st,
-  st ==[ skip2 ]=> st. (* = st =[ skip]=> st. *)
+  where "st ==[ c ]=> st'" := (ceval2 c st st').
+
+Theorem der_skip : forall st,
+  st =[ skip ]=> st <-> st ==[ skip2 ]=> st.
 Proof.
   intros.
-  apply E_CDo.
-  trivial.
+  split.
+  - intros. apply E_Do.
+  - intros. apply E_Skip.
 Qed.
 
-Theorem der_assign: forall st s a,
-  st ==[ assgn2 s a ]=> (s !-> (aeval st a) ; st).
+Theorem der_assign : forall st st' s a n,
+  (aeval st a) = n ->
+  st ==[s ::= n]=> st' <-> st =[s := n]=> st'.
 Proof.
   intros.
-  apply E_CDo.
-  trivial.
+  Print E_Asgn.
+  split.
+  - intros. inversion H0; subst. apply E_Asgn. trivial.
+  - intros. inversion H0; subst. apply E_Do.
 Qed.
 
 Definition Assertion := state -> Prop.
-Definition valid_hoare_triple
+
+Definition valid_hoare_triple2
            (P : Assertion) (c : com2) (Q : Assertion) : Prop :=
   forall st st',
      st ==[ c ]=> st' ->
      P st  ->
      Q st'.
 
-Notation "{{ P }} c {{ Q }}" := (valid_hoare_triple P c Q) (at level 90, c custom com at level 99).
-Check ({{fun st => True}} skip2  {{fun st => True}}).
+Notation "-{{ P }} c {{ Q }}-" :=
+  (valid_hoare_triple2 P c Q)
+    (at level 90, c custom com at level 99).
+Check (-{{fun st => True}} X ::= 0 {{fun st => True}}-).
 
-Theorem hoare_do : forall Q f (st : state),
-     {{ fun st => Q (f(st)) }} CDo f {{ Q }}.
+Example assertion_test :
+  -{{fun st => True}} X ::= 1 {{fun st => (st X) = 1}}-.
 Proof.
-  intros.
-  unfold valid_hoare_triple.
+  unfold valid_hoare_triple2.
   intros.
   inversion H; subst.
-  trivial.
-Qed.
 
-Example assertion_true_x1 :
-  {{fun st => True}} assgn2 X 2 {{fun st => (st X) = 2}}.
-Proof.
-  unfold valid_hoare_triple.
-  intros.
-  inversion H; subst.
-  trivial.
-Qed.
+
+
+
+
+
+
+
+
+
+
+
+
+
+
+
+
+
+
+
+
+
+
+
+
+
+
+
+
+
+(* Print state. *)
+(**)
+(* Inductive com2 : Type := *)
+(*   | CDo (f : (state -> state)) *)
+(*   (* | CSkip *) *)
+(*   (* | CAsgn (x : string) (a : aexp) *) *)
+(*   | CSeq (c1 c2 : com2) *)
+(*   | CIf (b : bexp) (c1 c2 : com2) *)
+(*   | CWhile (b : bexp) (c : com2). *)
+(**)
+(* Definition skip2 := CDo (fun st => st). *)
+(* Definition assgn2 (s: string) (a: aexp) := CDo (fun st => s !-> (aeval st a) ; st). *)
+(**)
+(* Reserved Notation *)
+(*   "st '==[' c ']=>' st'" *)
+(*   (at level 40, c custom com at level 99, *)
+(*   st constr, st' constr at next level). *)
+(**)
+(* Inductive ceval2 : com2 -> state -> state -> Prop := *)
+(*   (* | E_Skip : forall st, *) *)
+(*   (*     st =[ skip ]=> st *) *)
+(*   (* | E_Asgn  : forall st a n x, *) *)
+(*   (*     aeval st a = n -> *) *)
+(*   (*     st =[ x := a ]=> (x !-> n ; st) *) *)
+(*   | E_CDo : forall f st st', *)
+(*       st' = f st -> *)
+(*       st ==[ CDo f ]=> st' *)
+(*   | E_Seq : forall c1 c2 st st' st'', *)
+(*       st  ==[ c1 ]=> st'  -> *)
+(*       st' ==[ c2 ]=> st'' -> *)
+(*       st  ==[ CSeq c1 c2 ]=> st'' *)
+(*   | E_IfTrue : forall st st' b c1 c2, *)
+(*       beval st b = true -> *)
+(*       st ==[ c1 ]=> st' -> *)
+(*       st ==[ CIf b c1 c2 ]=> st' *)
+(*   | E_IfFalse : forall st st' b c1 c2, *)
+(*       beval st b = false -> *)
+(*       st ==[ c2 ]=> st' -> *)
+(*       st ==[ CIf b c1 c2 ]=> st' *)
+(*   | E_WhileFalse : forall b st c, *)
+(*       beval st b = false -> *)
+(*       st ==[ CWhile b c ]=> st *)
+(*   | E_WhileTrue : forall st st' st'' b c, *)
+(*       beval st b = true -> *)
+(*       st  ==[ c ]=> st' -> *)
+(*       st' ==[ CWhile b c ]=> st'' -> *)
+(*       st  ==[ CWhile b c ]=> st'' *)
+(*     where "st ==[ c ]=> st'" := (ceval2 c st st'). *)
+(**)
+(* Theorem der_skip: forall st, *)
+(*   st ==[ skip2 ]=> st. (* = st =[ skip]=> st. *) *)
+(* Proof. *)
+(*   intros. *)
+(*   apply E_CDo. *)
+(*   trivial. *)
+(* Qed. *)
+(**)
+(* Theorem der_assign: forall st s a, *)
+(*   st ==[ assgn2 s a ]=> (s !-> (aeval st a) ; st). *)
+(* Proof. *)
+(*   intros. *)
+(*   apply E_CDo. *)
+(*   trivial. *)
+(* Qed. *)
+(**)
+(* Definition Assertion := state -> Prop. *)
+(* Definition valid_hoare_triple *)
+(*            (P : Assertion) (c : com2) (Q : Assertion) : Prop := *)
+(*   forall st st', *)
+(*      st ==[ c ]=> st' -> *)
+(*      P st  -> *)
+(*      Q st'. *)
+(**)
+(* Notation "{{ P }} c {{ Q }}" := (valid_hoare_triple P c Q) (at level 90, c custom com at level 99). *)
+(* Check ({{fun st => True}} skip2  {{fun st => True}}). *)
+(**)
+(* Theorem hoare_do : forall Q f (st : state), *)
+(*      {{ fun st => Q (f(st)) }} CDo f {{ Q }}. *)
+(* Proof. *)
+(*   intros. *)
+(*   unfold valid_hoare_triple. *)
+(*   intros. *)
+(*   inversion H; subst. *)
+(*   trivial. *)
+(* Qed. *)
+(**)
+(* Example assertion_true_x1 : *)
+(*   {{fun st => True}} assgn2 X 2 {{fun st => (st X) = 2}}. *)
+(* Proof. *)
+(*   unfold valid_hoare_triple. *)
+(*   intros. *)
+(*   inversion H; subst. *)
+(*   trivial. *)
+(* Qed. *)
 
